bidirectional compatibility of pts_to; an equivalence lemma; a nd split and gather actions in heap

ulib/experimental/Steel.PCM.Reference.fst
@@ -37,28 +37,16 @@ val sl_admit (#a:_) (#p:_) (q:a -> slprop)
 
 
 assume
-val sl_admit_atomic (#a:_) (#uses:_) (#o:_) (#p:_) (q:a -> slprop)
+val sl_admit_atomic (#a:_) (#uses:_) (#p:_) (o:_) (q:a -> slprop)
   : SteelAtomic a uses o p q
-
-let read r =
-  let x = H.read r in
-  Basics.return (U.downgrade_val x)
-
-let lift_q #a (q:a -> slprop) : U.raise_t a -> slprop = fun v -> q (U.downgrade_val v)
-
-// let h_exists #a (p:a -> slprop) =
-//   h_forall #slprop (fun (q:slprop) ->
-//   h_forall (fun (x:a) -> p x `wand` q) `wand` q)
-
-// val elim_h_exists (#a:_) (p:a -> slprop) (q:slprop)
-//   : SteelT unit (h_exists p)
-//                 (fun _ -> h_forall (fun (x:a) -> p x `wand` q) `wand` q)
 
 
 assume
 val elim_h_exists (#a:_) (p:a -> slprop) (q:slprop { forall m (x:a). interp (p x) m ==> interp q m} )
   : SteelT unit (h_exists p)
                 (fun _ -> q)
+
+let lift_q #a (q:a -> slprop) : U.raise_t a -> slprop = fun v -> q (U.downgrade_val v)
 
 let lift_h_exists (#a:_) (p:a -> slprop)
   : SteelT unit (h_exists p)
@@ -69,6 +57,32 @@ let h_exists_cong (#a:_) (p:a -> slprop) (q:a -> slprop {forall x. equiv (p x) (
   : SteelT unit (h_exists p)
                 (fun _ -> h_exists q)
   = sl_admit _
+
+module A = Steel.PCM.Effect.Atomic
+let lift_h_exists_atomic (#a:_) #u (p:a -> slprop)
+  : SteelAtomic unit u unobservable
+                (h_exists p)
+                (fun _a -> h_exists #(U.raise_t a) (lift_q p))
+  = sl_admit_atomic unobservable _
+
+let h_exists_cong_atomic (#a:_) #u (p:a -> slprop) (q:a -> slprop {forall x. equiv (p x) (q x) })
+  : SteelAtomic unit u unobservable
+                (h_exists p)
+                (fun _ -> h_exists q)
+  = sl_admit_atomic unobservable _
+
+let read r =
+  let x = H.read r in
+  Basics.return (U.downgrade_val x)
+
+// let h_exists #a (p:a -> slprop) =
+//   h_forall #slprop (fun (q:slprop) ->
+//   h_forall (fun (x:a) -> p x `wand` q) `wand` q)
+
+// val elim_h_exists (#a:_) (p:a -> slprop) (q:slprop)
+//   : SteelT unit (h_exists p)
+//                 (fun _ -> h_forall (fun (x:a) -> p x `wand` q) `wand` q)
+
 
 let read_refine #a #p q r =
   Basics.h_assert (h_exists (fun (v:a) -> pts_to r p v `star` q v));
@@ -90,9 +104,20 @@ let share r = H.share r
 
 let gather r = H.gather r
 
-let ghost_read_refine r q = sl_admit_atomic _
 
-let cas r v v_old v_new = sl_admit_atomic _
+let ghost_read_refine #a #uses #p r q =
+  A.h_assert_atomic (h_exists (fun (v:a) -> pts_to r p v `star` q v));
+  lift_h_exists_atomic (fun (v:a) -> pts_to r p v `star` q v);
+  A.h_assert_atomic (h_exists (fun (v:U.raise_t a) -> pts_to r p (U.downgrade_val v) `star` q (U.downgrade_val v)));
+  h_exists_cong_atomic (fun (v:U.raise_t a) -> pts_to r p (U.downgrade_val v) `star` q (U.downgrade_val v))
+                       (fun (v:U.raise_t a) -> H.pts_to r p v `star` lift_q q v);
+  A.h_assert_atomic (h_exists (fun (v:U.raise_t a) -> H.pts_to r p v `star` lift_q q v));
+  let x = H.ghost_read_refine r (lift_q q) in
+  A.h_assert_atomic (H.pts_to r p x `star` lift_q q x);
+  A.h_assert_atomic (pts_to r p (U.downgrade_val x) `star` q (U.downgrade_val x));
+  A.return_atomic (U.downgrade_val x)
+
+let cas r v v_old v_new = sl_admit_atomic observable _
 
 let raise_ref r p v = Basics.return r
 
